

Steady state PASEP

From the prism of 1D Magnetic Random Walks

E. Kovalenko*, S. Nechaev†

* MIPT, Moscow, Russia

† LPTMS, Universite Paris Sud, Orsay, France

kovalenko.elizavebeth@gmail.com

Abstract

The Totally Asymmetric Simple Exclusion Process (TASEP) is a stochastic process on a regular one-dimensional lattice with the following dynamics: each site i ($1 < i < N$) of a one-dimensional lattice of N sites is either occupied by particle ($\tau = 1$) or empty ($\tau = 0$). During every infinitesimal time interval dt , each particle in the system has a probability dt of jumping to the next site on its right (for all particles on sites $1 < i < N - 1$) if this neighboring site is empty. Furthermore, a particle is added at site $i = 1$ with probability αdt if site 1 is empty and a particle is removed from site N with probability βdt if this site is occupied. The matrix ansatz for such a model is Well-studied: $P_N(\tau_1, \dots, \tau_N) = \langle W | \prod_{i=1}^N (\tau_i D + (1 - \tau_i) E) | V \rangle$, where matrices E, D satisfy the following algebra: $DE = E + D$. The q -deformation of this algebra is **DE-qED=E+D**. We are interested in a model called **PASEP**, that satisfies this algebra.

1. PASEP ansatz

Consider the Partially Asymmetric Exclusion Process (PASEP) by determining it's transition rates matrices:

$$h_1 = \begin{pmatrix} -\alpha & \gamma \\ \alpha & \gamma \end{pmatrix}, \quad h_N = \begin{pmatrix} -\delta & \beta \\ \delta & -\beta \end{pmatrix}.$$

where the basis is $\{0, 1\}$ (that means, for example, $\{(0, \tau_2, \dots, \tau_N); (1, \tau_2, \dots, \tau_N)\}$ for h_1).

$$h = \begin{pmatrix} 0 & 0 & 0 & 0 \\ 0 & -q & p & 0 \\ 0 & q & -p & 0 \\ 0 & 0 & 0 & 0 \end{pmatrix}.$$

Where the basis is $\{(0, 0); (0, 1); (1, 0); (1, 1)\}$.

We are interested in **the steady-state**. In this model, the state is clearly determined by $\tau_i \in \{0, 1\}$, so all probabilities satisfy:

$$\begin{aligned} \frac{d}{dt} P_N(\tau_1, \dots, \tau_N) &= \sum_{\sigma_1} (h_1)_{\tau_1 \sigma_1} P_N(\sigma_1, \tau_2, \dots, \tau_N) + \\ &\sum_{i=1}^{N-1} \sum_{\sigma_i \sigma_{i+1}} (h_1)_{\langle \tau_i \tau_{i+1} \rangle (\sigma_i \sigma_{i+1})} P_N(\dots, \sigma_i, \sigma_{i+1}, \dots) + \\ &+ \sum_{\sigma_N} (h_N)_{\tau_N \sigma_N} P_N(\tau_1, \dots, \tau_{N-1}, \sigma_N) = 0. \end{aligned} \quad (1)$$

Rewrite (1) in recursive form

- The left boundary:

$$\sum_{\sigma_1} \dots = (2\tau_1 - 1) x_L P_{N-1}(\tau_2, \dots). \quad (2)$$

Where x_L is some combination of γ and α

- The middle:

$$\sum_{\sigma_i \sigma_{i+1}} \dots = -a(\tau_i, \tau_{i+1}) P_{N-1}(\dots, \tau_{i-1}, \tau_{i+1}, \dots) + a(\tau_{i+1}, \tau_i). \quad (3)$$

$$\text{Where } a(\tau, \tau') = \begin{cases} p, & (\tau, \tau') = (1, 0) \\ q, & (\tau, \tau') = (0, 1) \\ 0, & (\tau, \tau') = (0, 0)/(1, 1) \end{cases}.$$

- The right boundary:

$$\sum_{\sigma_N} \dots = -(2\tau_N - 1) x_R P_{N-1}(\tau_1, \dots, \tau_{N-1}). \quad (4)$$

Consider the following ansatz

$$f_N(\tau) = \langle W | \prod_{k=1}^N (\tau_k D + (1 - \tau_k) E) | V \rangle. \quad (5)$$

Substituting (2), (3), (4) into (5) we obtain the following

$$\begin{aligned} pDE - qED &= pE - qD, \\ -\alpha \langle W | E + \gamma \langle W | D &= -x \langle W |, \\ -\delta E | V \rangle + \beta D | V \rangle &= x | V \rangle. \end{aligned} \quad (6)$$

Note: the first in (6) is definitely demanded algebra **DE-qED=E+D** (up to a simple transformation)

Matrix realization

To obtain an exact matrix realization of algebra (6) let's recall a q -boson algebra

$$aa^\dagger - qa^\dagger a = 1.$$

With basis $|n\rangle$, $n = 0, 1, 2, \dots$, on which a and a^\dagger act as usual

$$\begin{aligned} a |n\rangle &= \sqrt{1 - q^n} |n - 1\rangle, \quad (n \geq 1), \quad a |0\rangle = 0, \\ a^\dagger &= \sqrt{1 - q^{n+1}} |n + 1\rangle. \end{aligned}$$

Therefore, required representation in operator and matrix form respectively

$$\begin{aligned} D &= a^\dagger + \frac{1}{1 - q} \mathbb{I}, \quad E = \frac{1}{1 - q} a + \frac{1}{1 - q} \mathbb{I} \quad (7) \\ D &= \begin{pmatrix} \frac{1}{1-q} & \sqrt{1-q^1} & 0 & 0 & \dots \\ 0 & \frac{1}{1-q} & \sqrt{1-q^2} & 0 & \dots \\ 0 & 0 & \frac{1}{1-q} & \sqrt{1-q^3} & \dots \\ \vdots & \vdots & \vdots & \ddots & \ddots \end{pmatrix}, \\ E &= \begin{pmatrix} \frac{1}{1-q} & 0 & 0 & 0 & \dots \\ \frac{\sqrt{1-q^1}}{1-q} & \frac{1}{1-q} & 0 & 0 & \dots \\ 0 & \frac{\sqrt{1-q^2}}{1-q} & \frac{1}{1-q} & 0 & \dots \\ 0 & 0 & \frac{\sqrt{1-q^3}}{1-q} & \frac{1}{1-q} & \dots \\ \vdots & \vdots & \vdots & \ddots & \ddots \end{pmatrix}. \end{aligned}$$

2. Mockin path view

Define the transfer-matrix of 1-D Mockin random-walk as $T = D + E$. Explicitly:

$$T = \begin{pmatrix} \frac{1}{1-q} & \sqrt{1-q^1} & 0 & 0 & \dots \\ \frac{\sqrt{1-q^1}}{1-q} & \frac{1}{1-q} & \sqrt{1-q^2} & 0 & \dots \\ 0 & \frac{\sqrt{1-q^2}}{1-q} & \frac{1}{1-q} & \sqrt{1-q^3} & \dots \\ \vdots & \vdots & \vdots & \ddots & \ddots \end{pmatrix}, \quad (8)$$

In terms of Mockin path it means that the rates of moving up, down and horizontally (u_h, d_h and f_h respectively) are:

$$\begin{aligned} u_h &= T_{h,h+1} = \sqrt{1 - q^{h+1}}, \\ d_h &= T_{h,h-1} = \frac{\sqrt{1 - q^h}}{1 - q}, \quad (h \geq 1), \quad T_{0,-1} = 0, \\ f_h &= T_{h,h} = \frac{2}{1 - q}. \end{aligned}$$

This matrix may be symmetrized by transform $\tilde{T} = GTG^{-1}$, where $G = \text{diag}((1 - q)^{\frac{h}{2}})$.

Using Farvard's and spectral theorems, we may diagonalize \tilde{T} with the help of **continuous q-Hermite polynomials**

$$\tilde{T} \cong \left(\frac{2}{1 - q} \mathbb{I} + \frac{2}{\sqrt{1 - q}} M_x \right) \text{ on } L^2([-1, 1], d\mu(x)) \quad (9)$$

Where $U : l^2 \rightarrow L^2(\mu)$, $(Uf)(x) = \sum_{n \geq 0} f_n p_n(x)$

with $p_n(x) = \kappa_n H_n(x | q)$,

$$\frac{\kappa_{n+1}}{\kappa_n} = \frac{1}{1 - q^{n+1}}, \quad \frac{\kappa_{n-1}}{\kappa_n} = \sqrt{1 - q^n}.$$

The orthogonality measure:

$$d\mu(x) = \frac{1}{2\pi} \frac{w(x | q)}{\sqrt{1 - x^2}} dx.$$

Where

$$w(x | q) = \left| \left(e^{2i\theta} : q \right)_\infty \right|^2 = h(x, 1) h(x, -1) h \left(x, q^{\frac{1}{2}} \right) h \left(x, -q^{\frac{1}{2}} \right),$$

with

$$\begin{aligned} h(x, \alpha) &:= \prod_{k=0}^{\infty} \left[1 - 2\alpha x q^k + \alpha^2 q^{2k} \right] = \left(\alpha e^{i\theta}, \alpha e^{-i\theta}, q \right)_\infty, \\ x &= \cos \theta. \end{aligned}$$

3. The phase diagram

How boundary conditions – 2 last eq. in (6) – affect the matrix representation of algebra?

Note that the representation that we are going to assume is just one of many possible ones.

We will use the following notation:

$$\begin{aligned} \langle W | n \rangle &= w_n, \quad |n\rangle = 0, 1, 2, \dots, \\ \langle n | V \rangle &= v_n. \end{aligned}$$

We will demand (7) stay the same, therefore:

$$\begin{aligned} w_{n+1} &= \frac{\gamma}{\alpha} (1 - q) \sqrt{\frac{1 - q^n}{1 - q^{n+1}}} w_{n-1} + \frac{1 - (\alpha - \gamma)}{\alpha \sqrt{1 - q^{n+1}}} w_n, \\ v_{n+1} &= \frac{\delta}{\beta} \frac{1}{(1 - q)} \sqrt{\frac{1 - q^n}{1 - q^{n+1}}} v_{n-1} + \frac{1 - (\beta - \delta)}{\beta (1 - q) \sqrt{1 - q^{n+1}}} v_n. \end{aligned} \quad (10)$$

The phase transition occurs in the poles of $\langle W | T^N | V \rangle$. Using (9) we obtain:

$$\langle W | T^N | V \rangle = \int_{-1}^1 \left(\frac{2}{1 - q} + \frac{2}{\sqrt{1 - q}} x \right)^N \tilde{W}(x) \tilde{V}(x) d\mu(x).$$

Where $\tilde{W}(x) = \sum_{n \geq 0} (G^{-1} W)_n p_n(x)$, $\tilde{V}(x) = \sum_{n \geq 0} (GV)_n p_n(x)$.

If $q^n \rightarrow 0$ (n is large) our linear recursion on w_n, v_n (10) becomes constant, so $w_n \sim r^n$, $v_n \sim r^n$ for some r , therefore:

$$\begin{aligned} r^2 - Br - A(1 - q) &= 0, \\ r^2 - Dr - C &= 0. \end{aligned}$$

Where $A = \frac{\gamma}{\alpha}$, $B = \frac{1 - (\alpha - \gamma)}{\alpha}$, $C = \frac{\delta}{\beta(1 - q)}$, $D = \frac{1 - (\beta - \delta)}{\beta(1 - q)}$.

Let us denote $x_{eff} = \frac{r + r^{-1}}{2}$, then the phase transition occurs when $x_{eff} = \pm 1$, or equally $r = \pm 1$.

Then we analyze asymptotics of an integral, using the Laplace method:

- $\alpha > \frac{1 + \gamma(2 - q)}{2} \curvearrowright \beta > \frac{1 + 2\delta}{2 - q} \rightarrow \nu = \frac{3}{2}$,
- $\alpha < \frac{1 + \gamma(2 - q)}{2}$ and $\lambda_L > \max(\lambda(1), \lambda_R) \rightarrow \nu = \frac{1}{2}$,
- $\beta < \frac{1 + 2\delta}{2 - q}$ and $\lambda_R > \max(\lambda(1), \lambda_L) \rightarrow \nu = \frac{1}{2}$,
- $\alpha = \frac{1 + \gamma(2 - q)}{2}$ or $\beta = \frac{1 + 2\delta}{2 - q} \rightarrow \nu = \frac{1}{2}$,
- if both $\alpha = \frac{1 + \gamma(2 - q)}{2}$, $\beta = \frac{1 + 2\delta}{2 - q} \rightarrow \nu = 0$.

4. Hydrodynamic limit

In [1] Timo Seppalainen proves the formula for the flux function of a process with ergodic initial distribution and the expectation $\mathbb{E}(\eta(i, 0)) = \rho$

$$\begin{aligned} f(\rho) &= \lim_{t \rightarrow \infty} \frac{1}{t} \int_0^t \left[p \mathbb{P}(\eta(i, s) = 1, \eta(i + 1, s) = 0) - \right. \\ &\quad \left. - q \mathbb{P}(\eta(i, s) = 0, \eta(i + 1, s) = 0) \right]. \end{aligned} \quad (11)$$

One may show that $\nu_\rho(\eta_i = 1) = \rho$ is the invariant measure for such a process, i.e satisfies the condition: $\int Lf(\eta) \nu_\rho(d\eta) = 0 \quad \forall f \in C_0$. Therefore, we should substitute ν_ρ in (11) ($\nu_\rho = P_n$). Thus we get

$$f(\rho) = (p - q)\rho(1 - \rho).$$

Therefore, PDE:

$$\partial_t u + \partial_x((p - q)u(1 - u)) = 0.$$

Well-known results for other models:

1. TASEP

$$f(\rho) = \rho(1 - \rho).$$

2. q-TASEP

$$f_\alpha(\rho) = \alpha \cdot \rho, \quad \rho = \frac{\log q}{\log q + \log(1 - q) + \Psi_q(\log_q \alpha)}.$$

Where α is the parameter of the q -geometric distribution, $\Psi_q(z) = \frac{\partial}{\partial z} \log \Gamma_q(z)$

References

- [1] T. Seppalainen Existence of hydrodynamics for the totally asymmetric simple K-exclusion process. *Hydrodynamics for K-exclusion*, 361–415, 1999.
- [2] Patrik L. Ferrari and Bálint Veto Tracy–Widom asymptotics for q-TASEP. *Tracy–Widom asymptotics for q-TASEP*, Vol. 51, No. 4, 1465–1485, 2015.
- [3] Bernard Derrida, M. R. Evans, V. Hakim, V. Pasquier. Exact solution of a 1D asymmetric exclusion model using a matrix formulation. *Exact solution of an ASEP*, 1493–1517, 1993,
- [4] A. Valov, A. Gorsky, S. Nechaev. Equilibrium Mean-Field-Like Statistical Models with KPZ Scaling. *KPZ Scaling.*, 52(2), 185–201, 2021.
- [5] Roelof Koekoek, Peter A. Lesky, René F. Swarttouw. *Hypergeometric Orthogonal Polynomials and Their q-Analogues*. Hypergeometric Orthogonal Polynomials and Their q-Analogues, Springer, 2010.